Fix typeclass - finished

examples/cannon/CannonA.v
@@ -4,27 +4,23 @@ Require Import CannonHeader CannonASpec.
 
 Set Implicit Arguments.
 
-Module CannonA.
-Section A.
+Module CannonA. Section CannonA.
   Import CannonAS.
-  Context `{!sinvGS Σ Γ α β τ, !CannonAS.GS Γ}.
-  Local Notation iProp := (iProp Σ).
+  Context `{!invG α Σ Γ, !subHG Γ Σ, !sinvG Σ Γ α β τ, !CannonAGΓ Γ}.
 
   Definition scopes := ["Cannon"].
   Definition v_lv := "Cannon" ↯ "lv".
 
-  Definition fire: list val -> itree hmodE Z :=
-    fun _ =>
+  Definition fire : list val → itree hmodE Z :=
+    λ _,
       let r := 1%Z in
       _ <- trigger (@IO _ void "print" [r]↑);;
-      Ret r
-  .
+      Ret r.
 
   Definition fnsems :=
     [(CannonName.fire, (scopes, mk_specbody CannonAS.fire_spec (cfunU fire)))].
 
-  Program Definition Sem: SModSem.t :=
-  {|
+  Program Definition Sem : SModSem.t := {|
     SModSem.scopes := scopes;
     SModSem.fnsems := fnsems;
     SModSem.initial_st := [(v_lv, 1%Z↑)];
@@ -32,18 +28,15 @@ Section A.
   Solve All Obligations with prove_scope.
   Next Obligation. prove_nodup. Qed.
 
-  Definition Mod: SMod.t :=
-  {|
+  Definition Mod : SMod.t := {|
     SMod.modsem := fun _ => Sem;
     SMod.sk := CannonSK.t;
   |}.
 
-  Definition InitCond : Sk.t -> iProp :=
-    fun _ => Ready%I.
+  Definition InitCond : Sk.t → iProp Σ :=
+    λ _, Ready.
 
-  Variable ginv: Sk.t -> invspec.
-  Variable GlobalStb: Sk.t -> gname -> option fspec.
+  Variable ginv : Sk.t → invspec.
+  Variable GlobalStb : Sk.t → gname → option fspec.
   Definition t := Seal.sealing "ccr" (SMod.to_hmod ginv GlobalStb Mod).
-
-End A.
-End CannonA.
+End CannonA. End CannonA.
