examples/cannon/CannonASpec.v
@@ -5,63 +5,45 @@ Require Import CannonHeader.
 
 Set Implicit Arguments.
 
-Module CannonAS.
-Section CannonAS.
-  Local Definition RA : ucmra :=
-    excl_authR unitO.
-  Class GpreΓ (Γ : HRA) := {
-    #[global] map_inG :: inG (excl_authR unitO) Γ;
-  }.
-  Class GS (Γ: HRA) := {
-    #[global] RA_inG :: inG CannonAS.RA Γ;
-    map_name : positive;
-  }.
-  Definition GΓ : HRA := #[excl_authR unitO].
-  Global Instance subG_GΓ {Γ} : subG GΓ Γ → GpreΓ Γ.
-  Proof. solve_inG. Qed.
+Local Definition RA : ucmra := excl_authR unitO.
+Class CannonAGΓ (Γ : HRA) := {
+  #[local] map_inG :: inG (excl_authR unitO) Γ;
+}.
+Definition CannonAΓ : HRA := #[excl_authR unitO].
+Global Instance subG_GΓ {Γ : HRA} : subG CannonAΓ Γ → CannonAGΓ Γ.
+Proof. solve_inG. Qed.
 
-  Context `{!sinvGS Σ Γ α β τ, !CannonAS.GS Γ}.
-
+Module CannonAS. Section CannonAS.
+  Context `{!invG α Σ Γ, !subHG Γ Σ, !sinvG Σ Γ α β τ, !CannonAGΓ Γ}.
   
-  Definition Ready: iProp Σ := own map_name (●E tt).
-  Definition Ball: iProp Σ := own map_name (◯E tt).
-  Definition Fired: iProp Σ := own map_name ((●E tt) ⋅ (◯E tt)).
+  Definition Ready : iProp Σ := own 1%positive (●E tt).
+  Definition Ball : iProp Σ := own 1%positive (◯E tt).
+  Definition Fired : iProp Σ := own 1%positive ((●E tt) ⋅ (◯E tt)).
 
-  Lemma ReadyBall: 
-    Ready ∗ Ball ⊢ Fired.
+  Lemma ReadyBall : Ready ∗ Ball ⊢ Fired.
+  Proof. rewrite /Ready /Ball /Fired. iIntros "[B W]". iSplitL "B"; iFrame. Qed.
+
+  Lemma FiredReady : Ready ∗ Fired ⊢ False.
   Proof.
-    rewrite /Ready /Ball /Fired. unseal "CannonA".
-    iIntros "[B W]". iSplitL "B"; iFrame.
-  Qed.
-
-  Lemma FiredReady: 
-    Ready ∗ Fired ⊢ False.
-  Proof. 
-    rewrite /Ready /Fired. unseal "CannonA".
-    iIntros "[B0 [B1 W]]". iCombine "B0 B1" as "X" gives %FALSE.
+    rewrite /Ready /Fired. iIntros "[B0 [B1 W]]". iCombine "B0 B1" as "X" gives %FALSE.
     rewrite excl_auth_auth_op_valid // in FALSE.
   Qed.
 
-  Lemma FiredBall: 
-    Ball ∗ Fired ⊢ False.
+  Lemma FiredBall : Ball ∗ Fired ⊢ False.
   Proof.
-    rewrite /Ball /Fired. unseal "CannonA".
-    iIntros "[W0 [B W1]]". iCombine "W0 W1" as "X" gives %FALSE.
+    rewrite /Ball /Fired. iIntros "[W0 [B W1]]". iCombine "W0 W1" as "X" gives %FALSE.
     rewrite excl_auth_frag_op_valid // in FALSE.
   Qed.
 
-  Definition fire_spec: fspec :=
-    fspec_simple (fun (_: unit) =>
-        ((fun varg => (⌜varg = ([]: list val)↑⌝ ∗ Ball)%I),
-        (fun vret => (⌜vret = (1: Z)%Z↑⌝)%I))).
+  Definition fire_spec : fspec :=
+    fspec_simple (λ _ : unit,
+      ((λ arg, (⌜arg = ([]: list val)↑⌝ ∗ Ball)),
+      (λ ret, (⌜ret = (1: Z)%Z↑⌝)))
+    )%I.
 
-  Definition Stb: alist gname fspec :=
+  Definition Stb : alist gname fspec :=
     Seal.sealing "ccr" [(CannonName.fire, fire_spec)].
 
-  Lemma Stb_nodup: List.NoDup (List.map fst Stb).
-  Proof.
-    unfold Stb. unseal "ccr". prove_nodup.
-  Qed.
-
-End CannonAS.
-End CannonAS.
+  Lemma Stb_nodup : List.NoDup (List.map fst Stb).
+  Proof. unfold Stb. unseal "ccr". prove_nodup. Qed.
+End CannonAS. End CannonAS.
