examples/cannon/CannonI.v
@@ -2,38 +2,31 @@ Require Import CRIS.
 Require Import ImpPrelude.
 Require Import CannonHeader.
 
-
-Require Import sProp sWorld SRF.
-From stdpp Require Import coPset gmap namespaces.
-
 Set Implicit Arguments.
 
-Module CannonI.
-Section I.
+Module CannonI. Section CannonI.
   Local Open Scope string_scope.
-  (* Context `{sInvGS Σ Γ α β τ}. *)
+
   Context `{Σ: GRA}.
 
   Definition scopes := ["Cannon"].
   Definition v_lv := "Cannon" ↯ "lv". (* local variable *)
 
-  Definition div (n m: Z): option Z :=
+  Definition div (n m : Z) : option Z :=
     if Z_zerop m then None else Some (Z.div n m).
 
   Definition fire: list val -> itree pmodE Z :=
-    fun _ =>
+    λ _,
       powder <- cgetU v_lv;;
       r <- (div 1 powder)?;;
       _ <- trigger (@IO _ void "print" [r]↑);;
       cput v_lv (powder - 1)%Z;;;
-      Ret r
-  .
+      Ret r.
 
   Definition fnsems :=
     [(CannonName.fire, (scopes, cfunU fire))].
   
-  Program Definition Sem: PModSem.t :=
-  {|
+  Program Definition Sem : PModSem.t := {|
     PModSem.scopes := scopes;
     PModSem.fnsems := fnsems;
     PModSem.initial_st := [(v_lv, 1%Z↑)];
@@ -41,14 +34,10 @@ Section I.
   Solve All Obligations with prove_scope.
   Next Obligation. prove_nodup. Qed.
 
-  Definition Mod: PMod.t := 
-  {|
+  Definition Mod : PMod.t := {|
     PMod.modsem := fun _ => Sem;
     PMod.sk := CannonSK.t;
   |}.
 
   Definition t := Seal.sealing "ccr" (PMod.to_hmod Mod).
-
-End I.
-
-End CannonI.
+End CannonI. End CannonI.
