examples/cannon/CannonMainA.v
@@ -4,35 +4,30 @@ Require Import CannonHeader CannonMainASpec CannonMainI CannonASpec CannonHeader
 
 Set Implicit Arguments.
 
-Module MainA.
-Section A.
+Module MainA. Section MainA.
   Import CannonAS.
-  Context `{!sinvGS Σ Γ α β τ, !CannonAS.GS Γ}.
+  Context `{!invG α Σ Γ, !subHG Γ Σ, !sinvG Σ Γ α β τ, !CannonAGΓ Γ}.
 
-  Variable num_fire: nat.
+  Variable num_fire : nat.
 
   Definition scopes := ["Main"].
 
-  Fixpoint main_repeat (n: nat): itree hmodE unit :=
-  match n with
-  | 0 =>
-    Ret tt
-  | S n' =>
-    'r: Z <- ccallU CannonName.fire ([]: list val);;
-    _ <- trigger (@IO _ void "print" [r]↑);;
-    main_repeat n'
-  end.
+  Fixpoint main_repeat (n : nat) : itree hmodE unit :=
+    match n with
+    | 0 => Ret tt
+    | S n' =>
+      'r : Z <- ccallU CannonName.fire ([] : list val);;
+      _ <- trigger (@IO _ void "print" [r]↑);;
+      main_repeat n'
+    end.
 
-  Definition main: list val -> itree hmodE unit :=
-    fun _ =>
-      main_repeat num_fire
-  .
+  Definition main : list val → itree hmodE unit :=
+    λ _, main_repeat num_fire.
 
   Definition fnsems :=
     [(MainName.main, (scopes, mk_specbody CannonMainAS.main_spec (cfunU main)))].
 
-  Program Definition Sem: SModSem.t :=
-  {|
+  Program Definition Sem : SModSem.t := {|
     SModSem.scopes := scopes;
     SModSem.fnsems := fnsems;
     SModSem.initial_st := [];
@@ -40,18 +35,14 @@ Section A.
   Solve All Obligations with prove_scope.
   Next Obligation. prove_nodup. Qed.
 
-  Definition Mod: SMod.t :=
-  {|
-    SMod.modsem := fun _ => Sem;
+  Definition Mod : SMod.t := {|
+    SMod.modsem := λ _, Sem;
     SMod.sk := MainSK.t;
   |}.
 
-  Definition InitCond : Sk.t -> iProp Σ :=
-    fun _ => Ready%I.
+  Definition InitCond : Sk.t → iProp Σ := λ _, Ready.
 
-  Variable ginv: Sk.t -> invspec.
-  Variable GlobalStb: Sk.t -> gname -> option fspec.
+  Variable ginv : Sk.t → invspec.
+  Variable GlobalStb : Sk.t → gname → option fspec.
   Definition t := Seal.sealing "ccr" (SMod.to_hmod ginv GlobalStb Mod).
-
-End A.
-End MainA.
+End MainA. End MainA.
