examples/cannon/CannonMainI.v
@@ -4,35 +4,31 @@ Require Import CannonHeader.
 
 Set Implicit Arguments.
 
-Module MainI.
-Section I.
+Module MainI. Section MainI.
   Local Open Scope string_scope.
-  Context `{Σ: GRA}.
+
+  Context `{Σ : GRA}.
 
   Variable num_fire: nat.
 
   Definition scopes := ["Main"].
 
-  Fixpoint main_repeat (n: nat): itree pmodE unit :=
+  Fixpoint main_repeat (n : nat) : itree pmodE unit :=
     match n with
-    | 0 =>
-      Ret tt
+    | 0 => Ret tt
     | S n' =>
-      'r: Z <- ccallU CannonName.fire ([]: list val);;
+      'r : Z <- ccallU CannonName.fire ([] : list val);;
       trigger (@IO _ void "print" [r]↑);;;
       main_repeat n'
     end.
 
-  Definition main: list val -> itree pmodE unit :=
-    fun _ =>
-      main_repeat num_fire
-  .
+  Definition main : list val → itree pmodE unit :=
+    λ _, main_repeat num_fire.
 
   Definition fnsems :=
     [(MainName.main, (scopes, cfunU main))].
   
-  Program Definition Sem: PModSem.t :=
-  {|
+  Program Definition Sem : PModSem.t := {|
     PModSem.scopes := scopes;
     PModSem.fnsems := fnsems;
     PModSem.initial_st := [];
@@ -40,14 +36,10 @@ Section I.
   Solve All Obligations with prove_scope.
   Next Obligation. prove_nodup. Qed.
 
-  Definition Mod: PMod.t := 
-  {|
-    PMod.modsem := fun _ => Sem;
+  Definition Mod : PMod.t := {|
+    PMod.modsem := λ _, Sem;
     PMod.sk := MainSK.t;
   |}.
 
   Definition t := Seal.sealing "ccr" (PMod.to_hmod Mod).
-
-End I.
-
-End MainI.
+End MainI. End MainI.
