examples/cannon/CannonAll.v
@@ -2,52 +2,18 @@ Require Import CRIS.
 Require Import ImpPrelude.
 Require Import CannonIAproof CannonMainIAproof.
 Require Import CannonA CannonASpec CannonMainA CannonMainASpec .
-Require Import Cancellation.
+(* Require Import Cancellation. *)
 
 Set Implicit Arguments.
 
-Module CannonAll.
-Section C.
+Module CannonAll. Section CannonAll.
   Variable num_fire: nat.
-  Definition Γ : HRA := ##[invΓ; CannonAS.GΓ].
-  Local Existing Instance Γ.
-
-  Definition τ : Typ.t :=
-    fun _ => ST.t.
-  Local Existing Instance τ.
-
-  Definition α : SRFCons.t :=
-    fun n => 
-      match n with
-      | 0 => SL.syntax
-      | _ => inv_syntax
-      end.
-  Local Existing Instance α.
-
-  Definition Σ : GRA := ##[invΣ; Γ].
-  Local Existing Instance  Σ.
-
-  Local Instance subG_GΓ : subG Γ Σ.
-  Proof. Admitted. 
-
-  Local Instance invGS_GΓ: invGS Σ Γ.
-  Proof. Admitted.
-
-  Definition β : SRFIntp.t :=
-    fun n => 
-      match n with
-      | 0 => SL.t
-      | _ => (@inv_interp α Γ Σ subG_GΓ _) 
-      end.
-
-  Local Instance sinvGS_: sinvGS Σ Γ α β τ.
-  Proof. Admitted.
-
-  Local Instance asdf: CannonAS.GS Γ.
-  Proof. Admitted.
-
-  Definition Mod := (@CannonA.Mod Σ Γ α β τ sinvGS_ _) ☆ (@MainA.Mod Σ Γ α β τ sinvGS_ _ num_fire).
-
-
-End C.
-End CannonAll.
+  Import inv_instances.
+  Instance Γ : HRA := ##[invΓ; CannonAΓ].
+  Instance Σ : GRA := ##[invΣ; Γ].
+  
+  (* Set Typeclasses Debug Verbosity 2. *)
+  Set Typeclasses Depth 10.
+  (* Instance test : invG Σ Γ. eauto. apply _. *)
+  Definition Mod := (CannonA.Mod) ☆ (MainA.Mod num_fire).
+End CannonAll. End CannonAll.
