examples/cannon/CannonMainASpec.v
@@ -4,23 +4,19 @@ Require Import CannonHeader CannonASpec.
 
 Set Implicit Arguments.
 
-Module CannonMainAS.
-Section Main.
+Module CannonMainAS. Section CannonMainAS.
   Import CannonAS.
-  Context `{!sinvGS Σ Γ α β τ, !CannonAS.GS Γ}.
+  Context `{!invG α Σ Γ, !subHG Γ Σ, !sinvG Σ Γ α β τ, !CannonAGΓ Γ}.
 
   Definition main_spec: fspec :=
-    fspec_simple (fun (_: unit) =>
-        ((fun varg => (⌜varg = ([]: list val)↑⌝ ∗ Ball)%I),
-        (fun vret => (⌜vret = tt↑⌝)%I))).
+    fspec_simple (λ _ : unit,
+      ((λ arg, ⌜arg = ([]: list val)↑⌝ ∗ Ball),
+      (λ ret, ⌜ret = tt↑⌝))
+    )%I.
 
-  Definition Stb: alist gname fspec :=
+  Definition Stb : alist gname fspec :=
     Seal.sealing "ccr" [(MainName.main, main_spec)].
 
-  Lemma Stb_nodup: List.NoDup (List.map fst Stb).
-  Proof.
-    unfold Stb. unseal "ccr". prove_nodup.
-  Qed.
-
-End Main.
-End CannonMainAS.
+  Lemma Stb_nodup : List.NoDup (List.map fst Stb).
+  Proof. unfold Stb. unseal "ccr". prove_nodup. Qed.
+End CannonMainAS. End CannonMainAS.
